#Soma e Ativação
\(z = b + \sum_i w_i * x_i \)
\(y = \phi (z) = \frac{1}{1+e^{-z}}\)

#Gradiente
\(Gradiente: \frac{\partial\epsilon}{\partial w} = \frac{\partial E}{\partial y} \cdot \frac{\partial y}{\partial z} \cdot \frac{\partial z}{\partial w} \)

#Primeira Derivada Parcial
\(E^{saida} = \frac{1}{2} (g - y^{saida})^2 \)
\((g - y^{saida})^2 = \mu^2 \)
\(\epsilon = \frac{\partial E}{\partial y} = \frac{1}{2} \cdot 2(g-y^{saida}) \cdot \frac{d\mu}{dy} \) 
\(\epsilon = \frac{\partial E}{\partial y} = \frac{1}{2} \cdot 2(g-y^{saida}) \cdot -1 = -(g-y^{saida}) \)
\(\epsilon^{saida} = y^{saida}-g \)

#Segunda Derivada Parcial
\( y^{saida} = \phi(z^{saida}) = \frac{1}{1+e^{-z^{saida}}} \)
\(\frac{\partial y}{\partial z} = \frac{d\phi(z)}{dz} = \phi(z)(1-\phi(z)) \)
\(\delta^{saida} = y^{saida}(1-y^{saida}) \cdot \epsilon^{saida}\)

#Terceira Derivada Parcial 
\( \frac{d}{dz} = y^{saida} (1-y^{saida}) = \delta^{saida} \) 
\(\epsilon^{oculto} = y^{oculto}(1-y^{oculto})\)
\(\delta^{oculto} = \delta^{saida} \cdot w^{saida} \cdot \epsilon^{oculto}\)

#Ajustando os pesos
\(w_i^{saida} = w_i^{saida} - (\eta \cdot \delta^{saida} * y_i^{oculto}) \)
\(b_i^{saida} = b_i^{saida} - (\eta \cdot \delta^{saida})\)
\(w_i^{oculto} = w_i^{oculto} - (\mu \cdot \delta^{oculto} * x_i) \)
\(b_i^{oculto} = b_i^{oculto} - (\eta \cdot \delta^{oculto})\)